noc/EqnVect.v
@@ -1,0 +1,20 @@
+From Coq Require Import Arith Lia Program.
+From Equations Require Import Equations.
+
+Inductive index' {A} := thisone | anotherone (a: A).
+Arguments index': clear implicits.
+
+Equations index (n:nat) : Type :=
+    index 0 := False;
+    index (S n) := index' (index n).
+    
+
+Check False. 
+Compute index' False.
+
+Inductive rule_t := router_ (n:index 4).
+
+Compute router_ (thisone).
+
+
+
