noc/Interface.v
@@ -1,0 +1,35 @@
+Require Import Koika.Frontend.
+Require Import Koika.Std.
+Require Import Types.
+
+
+Module Interface.
+Import Types.
+
+Inductive reg_t:=
+| r1.
+
+Definition unwrap: UInternalFunction reg_t empty_ext_fn_t :=
+    {{ fun unwrap (packet: struct_t basic_flit) : bits_t 5 =>
+    let data := get(packet, data) in
+    data
+    }}.
+
+Definition wrap : UInternalFunction reg_t empty_ext_fn_t :=
+    {{ fun wrap (data: bits_t 5) (source: bits_t 4) (tx: bits_t 2)(ty: bits_t 2): struct_t basic_flit  =>
+    let packet := struct basic_flit
+            {
+             new := Ob~1;
+             src := source;
+             trg_x := tx;
+             trg_y := ty;
+             data := data
+            } in
+    data
+    }}.
+
+Print UInternalFunction.
+Print wrap.
+Print uaction.
+Check uaction.
+End Interface.
